wip

IterTree/Basic.lean
@@ -1,50 +1,225 @@
 namespace IterTree
 
-/-- iTree equivalent of Std.IterM -/
-structure iTree {σ : Type σ} («?» : Type r → Type q) (ρ : Type ρ) :
-    Type σ where
-  /-- I'm becoming more and more certian that this `iTree` definition
-  can be understood as a mapping between some program σ and both its
-  return type ρ and effects «?». These effects may depend on some type.-/
-  internalState : σ
+/-
+
+# What is an iTree?
+
+An iTree represents a computation. A computation can be represented by an infinitely
+branching tree, which give rise to the different possible traces.
+
+The type of an iTree is parametrized by two types:
+ - R, the type of values returned by the computation
+ - E, the possible events raised by the computation before it concludes. Data may be
+   requested by the computation before it can resume, and the event is allowed to 
+   depend on the type of this data.
+
+We would write this as 
+
+    coinductive iTree (E : Type → Type) (R : Type) where
+    | ret : R → iTree E R
+    | tau : iTree E R → iTree E R
+    | vis : ∀ A, E A → (A → iTree E R) → iTree E R
+
+However, in Lean we don't have coinductive data!
+
+We could talk about a finite version of iTrees though, if we just make the definition
+inductive.
+
+-/
+
+namespace Finite
+
+inductive iTree (E : Type q → Type r) (R : Type v) : Type _ where
+| ret : R → iTree E R
+| tau : iTree E R → iTree E R
+| vis {A : Type q} : E A → (A → iTree E R) → iTree E R
 
 /-
-The issue I see with our current API is that the internal program type is
-represented in our iTree interface, since its part of its type signature.
-This prevents us from having `iTree` have a nice monoidal interface, since
-an operation may transform the type of the internal state σ.
 
-For instance, we would like to implement the `return` combinator in our
-implementation, but this is represented by taking a new type `Return`,
-which can then be used by the typeclass resolution system to decide what
-the `exec` method is for our combinator. In a sense, we're defining a new
-instruction and giving its operational semantics through the `exec` method.
+Then, we can define a bunch of interesting operations over trees!
+
 -/
 
--- NOTE: We have that ι = σ
+namespace iTree
 
-/-- iTree equivalent of Std.IterStep 
+variable {E : Type q → Type r}
 
-These are the observable behaviours of an iTree of effects «?» and values ρ.
-We can also think about it as the possible ways to express the operational
-semantics of our program. It's either taking a step (given by `skip`), 
-producing a value (given by `done`), or asking for an interaction before it
-can proceed (given by `ask`). Or, in other words, executing some effect.
+def bindLeft {α β} (f : α → iTree E β) : iTree E α → iTree E β
+| .ret v    => f v
+| .tau it   => .tau (it.bindLeft f)
+| .vis ev k => .vis ev (fun a => (k a).bindLeft f)
+
+instance : Bind (iTree E) := ⟨(·.bindLeft ·)⟩
+instance : Pure (iTree E) := ⟨.ret⟩
+instance : Monad (iTree E) where
+instance  : LawfulMonad (iTree E) := .mk'
+   (id_map     := by intros α it; simp only [Functor.map, bind, pure, Function.comp_id]; induction it <;> simp [bindLeft, *] )
+   (pure_bind  := by intros α β it f; simp only [bind, bindLeft])
+   (bind_assoc := by intros α β γ it f g; simp only [bind]; induction it <;> simp [bindLeft, *])
+
+-- Defined as an inductive proposition, since we cannot test for equality of types (for the `vis`-`vis` case)
+inductive eqUpToTau : iTree E R → iTree E R → Prop where
+| of_ret (r : R) : (iTree.ret r).eqUpToTau (.ret r)
+| of_vis {A : Type q}(ev : E A) (k₁ k₂ : A → iTree E R) : (∀ a : A, (k₁ a).eqUpToTau (k₂ a)) → (iTree.vis ev k₁).eqUpToTau (.vis ev k₂)
+| of_tau (it₁ it₂ : iTree E R) : it₁.eqUpToTau it₂ → (iTree.tau it₁).eqUpToTau (.tau it₂)
+| of_left_tau (it₁ it₂ : iTree E R) : it₁.eqUpToTau it₂ → (iTree.tau it₁).eqUpToTau it₂
+| of_right_tau (it₁ it₂ : iTree E R) : it₁.eqUpToTau it₂ →  it₁.eqUpToTau (.tau it₂)
+
+/-
+
+The issue with this definition is that it cannot be used to capture most computations
+we're interested in. Without looking further, we cannot represent any computation which
+is infinite, like `loop {}`!
+
+Furthermore, the `tau` constructor in this definition is useless. It can always be
+stripped! In particular, our `eqUpToTau` predicate is equivalent to `Eq` if we run
+the iTrees we're comparing through our stripping function first.
+
 -/
-inductive Observation («?» : Type ι → Type q) (ρ : Type ρ) : Type _ where
-  | ask {α : Type ι}{σ : Type ι → Type ι} (ev : «?» α) (k : α → @iTree (σ α) «?» ρ) 
-  -- For now I allow our programs to depend on the type of events. 
-  | skip {σ : Type ι}(it : @iTree σ «?» ρ) 
-  | done (v : ρ) 
 
-/-- iTree equivalent of Std.Iterator 
+def stripTau : iTree E R → iTree E R 
+| .ret v => .ret v
+| .tau it => it.stripTau
+| .vis ev k => .vis ev (fun it => (k it).stripTau)
 
-It links implementations σ with iTrees of effects «?» and values ρ.
+theorem eqUpToTau_of_stripTau_eq_stripTau {it₁ it₂ : iTree E R} : (it₁.stripTau = it₂.stripTau) → it₁.eqUpToTau it₂ := by 
+  intros hyp
+  induction it₁ generalizing it₂ with
+  | ret v₁ =>
+    induction it₂ with 
+    | ret v₂ => 
+      grind [eqUpToTau, stripTau]
+    | tau it₂ => 
+      grind [stripTau, eqUpToTau]
+    | vis ev₂ k₂ => 
+      simp [stripTau] at hyp
+  | tau it₁ IH =>
+    grind [stripTau, eqUpToTau]
+  | vis ev₁ k₁ IH₁ =>
+    induction it₂ with 
+    | ret v₂ => 
+      grind [eqUpToTau, stripTau]
+    | tau it₂ => 
+      grind [stripTau, eqUpToTau]
+    | vis ev₂ k₂ IH₂ => 
+      simp [stripTau] at hyp
+      obtain ⟨rfl, rfl, hyp⟩ :=  hyp
+      simp only [heq_eq_eq] at hyp
+      replace hyp := fun a => congrFun hyp a
+      constructor
+      intros a 
+      apply IH₁
+      grind
+
+theorem eqUpToTau_iff_stripTau_eq_stripTau {it₁ it₂ : iTree E R} : it₁.eqUpToTau it₂ ↔ (it₁.stripTau = it₂.stripTau) := by 
+  constructor <;> intros hyp
+  · induction hyp <;> grind [stripTau]
+  · apply eqUpToTau_of_stripTau_eq_stripTau hyp
+
+end iTree
+
+end Finite
+
+
+/- 
+
+Therefore, we look to give a different presentation of iTrees, which does not have this problem, but also 
+allows definining the same operations as the finite case.
+
+-/ 
+
+namespace StateMachine
+
+/- 
+
+The first attempt I want to try is to give an encoding in terms of a state machine. Basically, we have a
+"current state" and a "step function" which tells us to what state to go next. 
+
+The issue with this representation is that a single, fixed state is not enough to express all we want out
+of iTrees (Is this actually true?).
+
+Inspired by Lean's Std.Iter APIs, we can attack a specific state with the ability to say it represents
+some `iTree`. In a sense, this means that we generalize over implementations of the `iTree`, to remain
+only with its interface, which is what we do theorems againsts.
+
 -/
-class Executable (σ : Type ι)
-  («?» : Type σ → Type q)
-  (ρ : Type ρ)
-where
-  IsPlausibleObservation : iTree (σ := σ) «?» ρ → Observation «?» ρ → Prop
-  exec : (it : iTree (σ := σ) «?» ρ) →
-    {obs : Observation «?» ρ // IsPlausibleObservation it obs}
+
+
+inductive Obs (E : Type q → Type r) (R : Type v) (K : Type k) where
+| ret : R → Obs E R K
+| tau : K → Obs E R K
+| vis {A : Type q} : E A → (A → K) → Obs E R K
+
+/- class IsITreeImpl (State : Type s) (E : Type q → Type r) (R : Type v) where -/
+/-     step : State → Obs E R State -/
+
+structure iTree (E : Type q → Type r) (R : Type v) where
+  {State : Type s}
+  curr : State
+  /- [stepImpl : IsITreeImpl State E R] -/
+  step : State → Obs E R (iTree E R)
+  -- Why not have it give observations on just `State`?
+  -- I think it's not possible, because we must be able to change
+  -- the state type at some point in the execution.
+  -- 
+  -- However, how do you define the infinitely looping
+  -- computation with `State → Obs E R (iTree E R)`?
+  -- You can't, you'd need to reference back to the think you're
+  -- defining, but at that point it's no longer a fixpoint!
+
+instance : Inhabited (iTree E R) where
+  default := {
+    State := Unit
+    curr := ()
+    step := fun _ => .tau 
+  }
+
+variable {E : Type q → Type r}{R : Type v}
+  
+
+def iTree.unfold (it : iTree E R) : Obs E R (iTree E R) := it.step it.curr 
+
+/-
+
+An alternate representation of this interface would be to have `curr : State` be the implementation of
+an `iTree E R`, and assign to each `State` type a particular `step` function.
+
+-/
+
+namespace iTree
+
+variable {E : Type q → Type r}
+
+/- instance : Inhabited ({E : Type q → Type r} → {α : Type u_1} → {β : Type u_2} → (α → iTree E β) → iTree E α → iTree E β) where -/
+/-   default f it := { -/
+    
+/-   } -/
+
+/--
+  After the computation of the interaction tree `it`, we simply continue with the
+  computation given by `f`. We encode the information of the continuation in the 
+  closure, to dodge problems with termination.
+-/
+partial
+def bindLeft {α β} (f : α → iTree E β)(it : iTree E α) : iTree E β :=
+  {
+    State := it.State
+    curr := it.curr
+    step st := match it.step st with
+      | .ret r => .tau (f r)
+      | .tau it => .tau (it.bindLeft f)
+      | .vis ev k => 
+        .vis ev (fun a => (k a).bindLeft f)
+  }
+
+/- instance : Bind (iTree E) := ⟨(·.bindLeft ·)⟩ -/
+/- instance : Pure (iTree E) := ⟨.ret⟩ -/
+/- instance : Monad (iTree E) where -/
+/- instance  : LawfulMonad (iTree E) := .mk' -/
+/-    (id_map     := by intros α it; simp only [Functor.map, bind, pure, Function.comp_id]; induction it <;> simp [bindLeft, *] ) -/
+/-    (pure_bind  := by intros α β it f; simp only [bind, bindLeft]) -/
+/-    (bind_assoc := by intros α β γ it f g; simp only [bind]; induction it <;> simp [bindLeft, *]) -/
+
+end iTree
+
+end StateMachine
